Main.lean
@@ -4,10 +4,10 @@ def bool_ty (A : Ty) : Ty := A -t> A -t> A
 
 def tt (A : Ty) : Term := :λ[A] :λ[A] #1
 def ff (A : Ty) : Term := :λ[A] :λ[A] #0
-def not (A : Ty) : Term := :λ[bool_ty (bool_ty A)] #0 :@ (ff A) :@ (tt A)
+def not (A : Ty) : Term := ((:λ[bool_ty (bool_ty A)] #0) :@ (ff A)) :@ (tt A)
 
-#eval Option.get! (infer .nil (tt ⊤))
-#eval Option.get! (infer .nil (not ⊤))
-#eval Option.get! (infer .nil ((not ⊤) :@ (tt (bool_ty ⊤))))
+#eval (infer .nil (tt ⊤))
+#eval (infer .nil (not ⊤))
+#eval (infer .nil ((not ⊤) :@ (tt (bool_ty ⊤))))
 
 def main : IO Unit := do return ()
